aa

Workbench.v
@@ -144,60 +144,36 @@ Proof.
     apply H. apply hs.
 Qed.
 
+(* Unique Atomic Names *)
+
+Fixpoint uniq_circ_syn {n : nat} (t : sterm n) (a : nat) : (sterm n * nat) :=
+match t with
+| SAbs t' => 
+  let (tnew, a') := uniq_circ_syn t' a in
+  (SAbs tnew, a')
+| SCir _ t' =>
+  let (tnew, a') := uniq_circ_chk t' (S a) in
+  (SCir a tnew, a')
+end
+with uniq_circ_chk {n : nat} (t : cterm n) (a : nat) : (cterm n * nat) :=
+match t with
+| CVar => (CVar, a)
+| CApp t1 t2 =>
+  let (tnew1, a1) := uniq_circ_chk t1 a in
+  let (tnew2, a2) := uniq_circ_syn t2 a1 in
+  (CApp tnew1 tnew2, a2)
+| CSqu t' =>
+  let (tnew, a') := uniq_circ_syn t' a in
+  (CSqu tnew, a')
+end.
+
+Definition uniq_circ {n : nat} (t : lterm n) : lterm n :=
+match t with
+| LSyn st => let (res, _) := uniq_circ_syn st 0 in LSyn res
+| LChk ct => let (res, _) := uniq_circ_chk ct 0 in LChk res
+end.
+
 (* Unification *)
-
-(*
-Theorem bidir_subst_syn :
-  forall {n : nat} (gamma : context n) (st : sterm n) (ty : type) (const : constraints) (sigma1 sigma2 : s_rules),
-  is_bidir_syn gamma st ty const ->
-  sat_xi sigma1 const ->
-  Permutation sigma1 sigma2 ->
-  sat_xi sigma2 const
-
-with bidir_subst_chk :
-  forall {n : nat} (gamma : context n) (ct : cterm n) (ty : type) (const : constraints) (sigma1 sigma2 : s_rules),
-  is_bidir_chk gamma ct ty const ->
-  sat_xi sigma1 const ->
-  Permutation sigma1 sigma2 ->
-  sat_xi sigma2 const.
-Proof.
-- intros n gamma st ty const sigma1 sigma2 hb hs hp.
-  induction hb.
-  + apply IHhb. apply hs.
-  + apply bidir_subst_chk with
-    (n := n) (gamma := gamma)
-    (ct := ct) (ty := TVar a)
-    (sigma1 := sigma1).
-    apply H. apply hs. apply hp.
-- intros n gamma st ty const sigma1 sigma2 hb hs hp.
-  einduction hb.
-  + apply sat_nil.
-  + assert (sat_xi sigma1 const1).
-    apply appleft_sat_xi with (const2 := const2). apply hs.
-    assert (sat_xi sigma1 const2).
-    apply appright_sat_xi with (const1 := const1). apply hs.
-    assert (sat_xi sigma2 const1).
-    apply IHi. apply i. apply H0.
-    assert (sat_xi sigma2 const2).
-    apply bidir_subst_syn with
-    (n := m) (gamma := delta)
-    (st := st2) (ty := ty1)
-    (sigma1 := sigma1).
-    apply H. apply H1. apply hp.
-    apply app_sat_xi.
-    apply H2. apply H3.
-  + dependent destruction hs.
-    apply sat_cons.
-    apply bidir_subst_syn with
-    (n := n) (gamma := gamma)
-    (st := st) (ty := ty1)
-    (sigma1 := sigma).
-    apply H0. apply hs. apply hp.
-
-induction hp.
-* simpl. simpl in H. apply H.
-* simpl. simpl in H.
-*)
 
 Inductive build_subst : s_rules -> constraints -> Prop :=
 | build_nil : build_subst List.nil List.nil
@@ -286,169 +262,9 @@ induction h.
     apply sat_cons.
 *)
 
-(*
 
-(*
-Consider: 
-unif_extra      only when !=Nil
-unif_perm_sigma ..
-unif_perm_const ..
 
-unif_taut sigma ty const:
-  sat_xi sigma (List.cons (ty, ty) const) ->
-  sat_xi sigma const
-*)
-
-Inductive sat_xi : s_rules -> constraints -> Prop :=
-| unif_empty : sat_xi List.nil List.nil
-| unif_left (n : nat) (ty : type) sigma const :
-  sat_xi sigma const ->
-  sat_xi (List.cons (n, ty) sigma) (List.cons (TVar n, ty) const)
-| unif_right (n : nat) (ty : type) sigma const :
-  sat_xi sigma const ->
-  sat_xi (List.cons (n, ty) sigma) (List.cons (ty, TVar n) const)
-| unif_imp (tyl1 tyl2 tyr1 tyr2 : type) rul sigma const :
-  sat_xi (List.cons rul sigma) (List.cons (tyl2, tyr2) (List.cons (tyr1, tyl1) const)) ->
-  sat_xi (List.cons rul sigma) (List.cons (TImp tyl1 tyl2, TImp tyr1 tyr2) const)
-| unif_skip rul sigma const :
-  sat_xi sigma const -> sat_xi (List.cons rul sigma) const
-| unif_extra sigma eq const :
-  sat_xi sigma (List.cons eq const) -> sat_xi sigma const
-| unif_perm_sigma sigma1 sigma2 const :
-  sat_xi sigma1 const -> Permutation sigma1 sigma2 ->
-  sat_xi sigma2 const
-| unif_perm_const sigma const1 const2 :
-  sat_xi sigma const1 -> Permutation const1 const2 ->
-  sat_xi sigma const2.
-
-Lemma skipall_sat_xi : forall (sigma : s_rules), sat_xi sigma List.nil.
-Proof.
-intro sigma. induction sigma.
-- apply unif_empty.
-- apply unif_skip. apply IHsigma.
-Qed.
-
-Lemma appleft_sat_xi : forall (sigma : s_rules) (const1 const2 : constraints),
-  sat_xi sigma (List.app const1 const2) -> sat_xi sigma const1.
-Proof.
-induction const2.
-- rewrite List.app_nil_r. intro h. apply h.
-- intro h. apply IHconst2.
-  assert (Permutation (const1 ++ a :: const2)%list (a :: (const1 ++ const2))%list).
-  Check Permutation_cons_app.
-  apply (Permutation_sym (Permutation_cons_app
-    (l := (const1 ++ const2)) const1 const2 a
-    (Permutation_refl (const1 ++ const2)))).
-  assert (sat_xi sigma (a :: const1 ++ const2)%list).
-  apply (unif_perm_const sigma (const1 ++ a :: const2)%list (a :: (const1 ++ const2))%list).
-  apply h. apply H.
-  apply unif_extra with (eq := a).
-  apply H0.
-Qed.
-
-Lemma appright_sat_xi : forall (sigma : s_rules) (const1 const2 : constraints),
-  sat_xi sigma (List.app const1 const2) -> sat_xi sigma const2.
-Proof.
-induction const1.
-- simpl. intros const2 h. apply h.
-- intros const2 h. apply IHconst1.
-  simpl in h. apply unif_extra with (eq := a).
-  apply h.
-Qed.
-
-(* TODO *)
-Lemma nil_rules : forall (const : constraints) (ty1 ty2 : type),
-  sat_xi List.nil (List.cons (ty1, ty2) const) ->
-  ty1 <> ty2.
-Proof.
-intros const ty1 ty2 h.
-dependent induction h.
-- apply IHh with (const := const).
-Admitted.
-
-(* TODO *)
-Lemma subst_converge : forall (sigma : s_rules) (const : constraints) (ty1 ty2 : type),
-  sat_xi sigma ((ty1, ty2) :: const)%list ->
-  subst_ty sigma ty1 = subst_ty sigma ty2.
-Proof.
-intros sigma const ty1 ty2 h.
-induction sigma.
-- dependent destruction h.
-  + simpl. admit.
-  + simpl. destruct sigma1.
-    * admit.
-    * apply Permutation_sym in H.
-      assert (~Permutation Datatypes.nil (s :: sigma1))
-        by (apply (Permutation_nil_cons (l := sigma1) (x := s))).
-      apply H0 in H. contradiction.
-  + simpl. destruct const1.
-    * admit.
-    * admit.
-- dependent destruction h.
-Admitted.
-
-(* Theorem *)
-
-Theorem bidir_typed_syn :
-  forall {n : nat} (gamma : context n) (st : sterm n) (ty : type) (const : constraints) (sigma : s_rules),
-  is_bidir_syn gamma st ty const ->
-  sat_xi sigma const ->
-  is_typed (subst_ctx sigma gamma) (strip_syn st) (subst_ty sigma ty)
-
-with bidir_typed_chk :
-  forall {n : nat} (gamma : context n) (ct : cterm n) (ty : type) (const : constraints) (sigma : s_rules),
-  is_bidir_chk gamma ct ty const ->
-  sat_xi sigma const ->
-  is_typed (subst_ctx sigma gamma) (strip_chk ct) (subst_ty sigma ty).
-
-Proof.
-- intros n gamma st ty const sigma hb hs.
-  induction hb.
-  + simpl.
-    rewrite dist_subst_ty.
-    apply (
-      typed_abs
-      (subst_ty sigma ty1) (subst_ctx sigma gamma)
-      (strip_syn st) (subst_ty sigma ty2)
-    ).
-    rewrite <- cons_subst_ctx.
-    apply IHhb. apply hs.
-  + simpl. apply bidir_typed_chk with (const := const).
-    apply H. apply hs.
-- intros n gamma ct ty const sigma hb hs.
-  induction hb.
-  + simpl.
-    rewrite single_subst_ctx.
-    apply (typed_var (subst_ty sigma ty)).
-  + simpl.
-    rewrite app_subst_ctx.
-    apply (
-      typed_app
-      (subst_ctx sigma gamma) (subst_ctx sigma delta)
-      (strip_chk ct1) (strip_syn st2)
-      (subst_ty sigma ty1) (subst_ty sigma ty2)
-    ).
-    * rewrite <- dist_subst_ty.
-      apply IHhb.
-      apply appleft_sat_xi with (const2 := const2).
-      apply hs.
-    * apply bidir_typed_syn with (const := const2).
-      apply H.
-      apply appright_sat_xi with (const1 := const1).
-      apply hs.
-  + simpl.
-    assert (subst_ty sigma ty1 = subst_ty sigma ty2).
-    apply subst_converge with (const := const).
-    apply hs.
-    rewrite <- H0.
-    apply bidir_typed_syn with (const := const).
-    apply H.
-    apply unif_extra with (eq := (ty1, ty2)).
-    apply hs.
-Qed.
-*)
-
-(* TODO: Principal Typing *)
+(* Principal Typing *)
 
 Definition is_princ : Type := forall {n : nat} (ctx : context n) (pt : pterm n) (ty : type),
   is_typed ctx pt ty -> forall (ctx' : context n) (ty' : type), is_typed ctx' pt ty' ->
@@ -457,14 +273,77 @@ Definition is_princ : Type := forall {n : nat} (ctx : context n) (pt : pterm n) 
 
 
 
+(* ================== *)
 
 
+Inductive is_inter_syn : forall {a : nat}, context a -> sterm a -> type -> Prop :=
+| inter_abs {n} ty1 gamma (st : sterm (S n)) ty2 :
+  is_inter_syn (gamma :: ty1) st ty2 -> 
+  is_inter_syn  gamma (SAbs st) (TImp ty1 ty2)
+| inter_cir {n} (a : nat) gamma (ct : cterm n) sigma :
+  is_inter_chk gamma ct (TVar a) sigma ->
+  is_inter_syn (subst_ctx sigma gamma) (SCir a ct) (subst_ty sigma (TVar a))
+
+with is_inter_chk : forall {a : nat}, context a -> cterm a -> type -> s_rules -> Prop :=
+| inter_var ty : is_inter_chk [ty] CVar ty List.nil
+| inter_app {n m} gamma delta (ct1 : cterm n) (st2 : sterm m) ty1 ty2 sigma :
+  is_inter_chk gamma ct1 (TImp ty1 ty2) sigma ->
+  is_inter_syn delta st2 ty1 ->
+  is_inter_chk (gamma ++ delta) (CApp ct1 st2) ty2 sigma
+| inter_squ {n} gamma (st : sterm n) ty1 ty2 sigma :
+  is_inter_syn gamma st ty1 ->
+  sat_xi sigma ((ty1, ty2) :: List.nil)%list ->
+  is_inter_chk gamma (CSqu st) ty2 sigma.
+
+Inductive is_inter : forall {a : nat}, context a -> lterm a -> type -> Prop :=
+| Sbidir {n} gamma (st : sterm n) ty :
+  is_inter_syn gamma st ty ->
+  is_inter gamma (LSyn st) ty
+| Cbidir {n} gamma (ct : cterm n) ty :
+  is_inter_chk gamma ct ty List.nil ->
+  is_inter gamma (LChk ct) ty.
+
+(*
+Lemma inter_chk_sigma :
+  forall {n : nat} (gamma : context n) (ct : cterm n) (a : nat) (sigma : s_rules),
+  is_inter_chk gamma ct (TVar a) sigma ->
+  is_inter_chk (subst_ctx sigma gamma) ct (subst_ty sigma (TVar a)) Datatypes.nil.
+Proof.
+intros n gamma ct a sigma h.
+induction h.
+- simpl. apply inter_var.
+- rewrite app_subst_ctx.
+  apply inter_app with (ty1 := subst_ty sigma ty1).
+  + rewrite <- dist_subst_ty.
+    apply IHh.
+  + 
+
+*)
+
+(*
+
+Definition is_princ : Type := forall {n : nat} (ctx : context n) (pt : pterm n) (ty : type),
+  is_typed ctx pt ty -> forall (ctx' : context n) (ty' : type), is_typed ctx' pt ty' ->
+  sig (fun (sigma : s_rules) => ctx' = subst_ctx sigma ctx /\ ty' = subst_ty sigma ty).
+
+*)
 
 
+Definition inter_typed_syn : Type :=
+  forall {n : nat} (gamma : context n) (st : sterm n) (ty : type),
+  is_inter_syn gamma st ty ->
+  sig (
+    fun (const : constraints) =>
+    is_bidir_syn gamma st ty const
+  ).
 
-
-
-
+Definition inter_typed_chk : Type :=
+  forall {n : nat} (gamma : context n) (ct : cterm n) (ty : type) (sigma : s_rules),
+  is_inter_chk gamma ct ty sigma ->
+  sig (
+    fun (const : constraints) =>
+    is_bidir_chk gamma ct ty const
+  ).
 
 
 
